theories/ltl_adequacy.v
@@ -1,60 +1,72 @@
-From ltl Require Import ltl ltl_fixpoints ltl_now.
+From ltl Require Import trace ltl ltl_fixpoints ltl_now.
 
 Section ltl_adequacy.
   Context {S L : Type}.
   Context {Rel : S → L → S → Prop}.
+  Notation tProp' := tProp.
   Notation tProp := (tProp S L Rel).
 
   Import tProp.
 
   Lemma ltl_adequate (P Q : tProp) :
-    (P ⊢ Q)%I ≡ (∀ tr, P tr → Q tr).
+    (P ⊢ Q)%I ≡ (∀ tr, trace_maximal Rel tr → P tr → Q tr).
   Proof.
     split.
-    - intros. apply H. done.
+    - intros ???. apply H. done.
     - intros. done.
   Qed.
 
   Lemma ltl_next_adequate (P : tProp) tr :
-    (○ P)%I tr ≡ P (wf_tail tr).
+    (○ P)%I tr ≡ P (tail_trace tr).
   Proof. rewrite ltl_next_unseal. done. Qed.
 
+  Lemma trace_tail_after (tr : trace S L) :
+    tail_trace tr = after 1 tr.
+  Proof. done. Qed.
+  
+  Lemma trace_tail_after_comm n (tr : trace S L) :
+    tail_trace (after n tr) = after n (tail_trace tr).
+  Proof. rewrite trace_tail_after after_sum_comm. done. Qed.
+
   Lemma ltl_next_iter_adequate n (P : tProp) tr :
-    (○^n P)%I tr ≡ P (wf_after n tr).
+    (○^n P)%I tr ≡ P (after n tr).
   Proof.
     revert tr P. induction n; intros tr P.
-    { simpl. rewrite wf_after_0. done. }
-    simpl. replace (Datatypes.S n) with (n + 1) by lia.
-    rewrite wf_after_sum.
-    rewrite ltl_next_adequate. rewrite -IHn. done.
+    { simpl. done. }
+    replace (Datatypes.S n) with (1 + n) by lia.
+    simpl.
+    rewrite trace_tail_after.
+    rewrite after_sum_comm.
+    rewrite ltl_next_adequate. 
+    rewrite IHn.
+    done.
   Qed.
 
+  Lemma ltl_always_equiv (P : tProp) :
+    (□ P)%I ≡ (∀ n, ○^n P)%I.
+  Proof. apply ltl_always_unseal'. Qed.
+
   Lemma ltl_always_adequate (P : tProp) tr :
-    (□ P)%I tr ≡ ∀ n, P (wf_after n tr).
+    (□ P)%I tr ≡ (∀ n, P (after n tr)).
   Proof.
     rewrite bi_intuitionistically_unseal'. rewrite ltl_always_unseal.
     rewrite /ltl_always_def. unseal.
     split.
-    - intros.
+    - intros H n.
       specialize (H n). simpl in *.
       revert P tr H.
       induction n; intros P tr H.
-      { simpl in *. rewrite wf_after_0. done. }
+      { simpl in *. done. }
       simpl in *. rewrite ltl_next_adequate in H.
       apply IHn in H.
-      (* rewrite -wf_after_sum in H. *)
       replace (Datatypes.S n) with (n + 1) by lia.
-      rewrite wf_after_sum. done.
+      rewrite trace_tail_after_comm. done.
     - intros H n.
       specialize (H n).
       revert tr P H.
       induction n; intros tr P H.
-      { simpl in *. rewrite wf_after_0 in H. done. }
-      apply ltl_next_iter_S.
-      apply IHn.
-      rewrite ltl_next_adequate.
-      replace (Datatypes.S n) with (1 + n) in H by lia.
-      rewrite wf_after_sum in H. done.
+      { simpl in *. done. }
+      apply ltl_next_iter_adequate. done.
   Qed.
 
   Lemma ltl_eventually_next_equiv (P : tProp) :
@@ -79,20 +91,21 @@ Section ltl_adequacy.
   Qed.
 
   (* TODO: Clean up this proof *)
-  Lemma ltl_eventually_adequate_1 (P : tProp) tr :
-    (∃ n, P (wf_after n tr)) → (◊ P)%I tr.
-  Proof. 
+  Lemma ltl_eventually_adequate_1 (P : tProp) tr (Hwf : trace_maximal Rel tr) :
+    (∃ n, P (after n tr)) → (◊ P)%I tr.
+  Proof.
     intros H.
-    apply ltl_eventually_next_equiv.
+    apply ltl_eventually_next_equiv; [done|].
     destruct H as [n Hn].
     unseal. exists n.
-    revert tr P Hn.
-    induction n; intros tr P Hn.
-    { rewrite wf_after_0 in Hn. simpl. done. }
-    apply ltl_next_iter_S. apply IHn.
+    revert tr P Hn Hwf.
+    induction n; intros tr P Hn Hwf.
+    { simpl. done. }
+    apply ltl_next_iter_S; [done|].
+    apply IHn; [|done].
     rewrite ltl_next_adequate.
     replace (Datatypes.S n) with (1+n) in Hn by lia.
-    rewrite wf_after_sum in Hn. done.
+    rewrite after_sum in Hn. done.
   Qed.
 
   Lemma ltl_eventually_adequate_2 (P : tProp) :
@@ -109,65 +122,65 @@ Section ltl_adequacy.
     done.
   Qed.
 
-  Lemma ltl_eventually_adequate (P : tProp) tr :
-    (◊ P)%I tr ≡ ∃ n, P (wf_after n tr).
+  Lemma ltl_eventually_adequate (P : tProp) tr (Hwf : trace_maximal Rel tr):
+    (◊ P)%I tr ≡ ∃ n, P (after n tr).
   Proof.
-    split; [|apply ltl_eventually_adequate_1].
+    split; [|by apply ltl_eventually_adequate_1].
     intros.
-    apply ltl_eventually_adequate_2 in H.
+    apply ltl_eventually_adequate_2 in H; [|done].
     revert H. unseal. intros H. destruct H as [n Hn].
-    revert tr Hn.
-    induction n; intros tr Hn.
-    { exists 0. by rewrite wf_after_0. }
+    revert tr Hn Hwf.
+    induction n; intros tr Hn Hwf.
+    { exists 0. done. }
     simpl in *.
     rewrite ltl_next_adequate in Hn.
-    apply IHn in Hn.
+    apply IHn in Hn; [|by apply wf_after_tail_wf].
     destruct Hn as [m Hn].
     exists (Datatypes.S m).
     replace (Datatypes.S m) with (m + 1) by lia.
-    rewrite wf_after_sum. done.
+    rewrite after_sum. done.
   Qed.
 
-  Lemma ltl_now_adequate P (tr : wf_trace S L Rel) :
-    (↓ P)%I tr ≡ P $ head_trace (tr_car tr).
+  Lemma ltl_now_adequate P (tr : trace S L) :
+    ((↓ P)%I:tProp) tr ≡ P $ head_trace tr.
   Proof.
     rewrite ltl_now_unseal. split.
     - intros. simplify_eq; done.
-    - intros. destruct tr as [[[]|]]; done.
+    - intros. destruct tr as [[]|]; done.
   Qed.
 
-  Lemma ltl_now_f_adequate {A} f (x : A) (tr : wf_trace S L Rel) :
-    (↓fs f x)%I tr ≡ (f <$> (fst <$> head_trace (tr_car tr)) = Some x).
+  Lemma ltl_now_f_adequate {A} f (x : A) (tr : trace S L) :
+    ((↓fs f x)%I:tProp) tr ≡ (f <$> (fst <$> head_trace tr) = Some x).
   Proof.
     rewrite ltl_now_adequate.
     split.
-    - intros. destruct tr as [[[]|]]; simpl in *; simplify_eq; try eauto; try done.
-    - intros. destruct tr as [[[]|]]; inversion H; simplify_eq; try eauto; try done.
+    - intros. destruct tr as [[]|]; simpl in *; simplify_eq; try eauto; try done.
+    - intros. destruct tr as [[]|]; inversion H; simplify_eq; try eauto; try done.
   Qed.
 
-  Lemma ltl_now_label_f_adequate {A} f (x : A) (tr : wf_trace S L Rel) :
-    (↓fl f x)%I tr ≡ (f <$> mjoin (snd <$> head_trace (tr_car tr)) = Some x).
+  Lemma ltl_now_label_f_adequate {A} f (x : A) (tr : trace S L) :
+    ((↓fl f x)%I:tProp) tr ≡ (f <$> mjoin (snd <$> head_trace tr) = Some x).
   Proof.
     rewrite ltl_now_adequate.
     split.
-    - intros. destruct tr as [[[]|]]; simpl in *; simplify_eq; try eauto; try done.
-    - intros. destruct tr as [[[]|]]; inversion H; simplify_eq; try eauto; try done.
+    - intros. destruct tr as [[]|]; simpl in *; simplify_eq; try eauto; try done.
+    - intros. destruct tr as [[]|]; inversion H; simplify_eq; try eauto; try done.
   Qed.
 
 End ltl_adequacy.
 
-Ltac adequacy_unseal_core := 
+Import tProp.
+
+Tactic Notation "adequacy_unseal" := 
   try rewrite !ltl_impl_unseal /ltl_impl_def;
   try rewrite !ltl_and_unseal /ltl_and_def;
-  try rewrite !ltl_always_adequate;
-  try rewrite ltl_next_unseal /ltl_next_def;
-  try setoid_rewrite ltl_eventually_adequate;
+  try setoid_rewrite ltl_always_equiv;
+  try setoid_rewrite ltl_eventually_next_equiv;
+  try rewrite !ltl_forall_unseal /ltl_forall_def;
+  try rewrite !ltl_exist_unseal /ltl_exist_def;
+  try rewrite ltl_adequate;
+  try setoid_rewrite ltl_next_adequate;
+  try setoid_rewrite ltl_next_iter_adequate;
   try setoid_rewrite ltl_now_f_adequate;
   try setoid_rewrite ltl_now_label_f_adequate;
   try setoid_rewrite ltl_now_adequate.
-
-Ltac adequacy_unseal :=
-  rewrite ltl_adequate; adequacy_unseal_core.
-
-Ltac adequacy_unseal_goal :=
-  rewrite ltl_adequate; try (intros ?tr); adequacy_unseal_core.
